hdr models

hdr.fst
@@ -2,11 +2,30 @@ module Hdr
 
 open FStar.Integers
 open FStar.Int
+open FStar.Int.Cast
+open FStar.Printf
 
-type point_ty = int
+let rm = 0x544f4952ul (*RIOTBOOT_MAGIC*)
 
-val rb_hdr_print : point_ty -> unit
+type rb_hdr_t = {magic_number : UInt32.t; 
+                 version : UInt32.t; 
+                 start_addr : UInt32.t; 
+                 chksum : UInt32.t}
 
-val rb_hdr_validate : point_ty -> int
+let rb_hdr_print (h: rb_hdr_t)  = 
+sprintf "Image magic_number: 0x%ul\n Image Version: 0x%ul\n Image start address: 0x%ul\n Header chksum: 0x%ul\n" h.magic_number h.version h.start_addr h.chksum
+(*\n? no 08 no multi sprintf statement*)
 
-val rb_hdr_checksum : point_ty -> UInt32.t
+val rb_hdr_checksum : rb_hdr_t -> UInt32.t
+
+open Fletcher32
+
+let rb_hdr_checksum h = Fletcher32.f32 0xd300us 6us (*here we give a random address, current version without pointers or memory models*)
+
+val rb_hdr_validate : rb_hdr_t -> int
+
+let rb_hdr_validate h =
+  if (h.magic_number = rm) && (rb_hdr_checksum(h) = h.chksum) then 
+    0
+  else 
+    -1
