fletcher32.fst
@@ -1,0 +1,82 @@
+module Fletcher32
+
+open FStar.Integers
+open FStar.Int
+open FStar.Int.Cast
+
+(*
+@original:
+do {
+     sum2 += sum1 += unaligned_get_u16(data++);
+} while (--tlen);
+=>(trans)
+
+do {
+  sum1 = sum1 + *(data++);
+  sum2 = sum2 + sum1;
+  tlen = tlen - 1;
+} while (tlen != 0)
+=> (to_caml)
+*)
+
+val dowhile : tlen:UInt32.t{tlen >= 0ul} -> UInt16.t -> UInt32.t -> UInt32.t -> Tot (UInt16.t & UInt32.t & UInt32.t) (decreases (v tlen))
+
+let rec dowhile tlen d s1 s2 =
+    match tlen with
+    | 0ul -> (d, (UInt32.add_mod s1 (UInt32.uint_to_t (UInt16.v d))), s2)
+    | _ ->        
+      let data =UInt16.add_mod d 16us in
+        let sum1 =UInt32.add_mod s1 (UInt32.uint_to_t (UInt16.v data)) in
+          let sum2 = UInt32.add_mod s2 sum1 in
+            dowhile (tlen - 1ul) data s1 s2
+(*
+@comment testing code
+
+val test1 : d:UInt16.t{size ((v d) + 1) 16} -> UInt32.t
+
+val test1 : d:UInt16.t{size ((v d) + (v 1us)) 16} -> UInt32.t
+
+
+let test1 d = 
+  let d1 = d + 1us in
+    assert (size (v d1) 16);
+    UInt32.uint_to_t (UInt16.v d1)
+
+val test2 : int -> (int & int)
+let test2 (d:int) = (d,d)
+*)
+
+(*
+@original:
+ uint32_t sum1 = 0xffff, sum2 = 0xffff;
+ while (words) {
+   unsigned tlen = words > 359 ? 359 : words;
+   words -= tlen; 
+   //...dowhile        
+   sum1 = (sum1 & 0xffff) + (sum1 >> 16);
+   sum2 = (sum2 & 0xffff) + (sum2 >> 16);
+ }     
+ sum1 = (sum1 & 0xffff) + (sum1 >> 16);
+ sum2 = (sum2 & 0xffff) + (sum2 >> 16);
+ *)
+
+val  while_t : (words : UInt16.t{words >= 0us}) -> UInt16.t -> UInt32.t -> UInt32.t -> Tot (UInt32.t & UInt32.t) (decreases (v words))
+
+let rec while_t words data s1 s2 =
+  match words with
+  | 0us -> (s1, s2)
+  | _ -> 
+    let tlen = if words > 359us then 359us else words in
+     assert (words >= 0us);
+     assert ((words - tlen) >= 0us);
+     assert (tlen >= 0us);     
+    let (data, sum1, sum2) = dowhile (uint16_to_uint32 tlen) data s1 s2 in
+    let sum11 = UInt32.add_mod (UInt32.logand sum1 0xfffful) (sum1 >>^ 16ul) in     
+    let sum21 = UInt32.add_mod (UInt32.logand sum2 0xfffful) (sum2 >>^ 16ul) in
+     while_t (UInt16.sub_mod words tlen) data sum11 sum21
+
+let f32 (data words : UInt16.t) =
+  let (sum1,sum2) = while_t words data 0xfffful 0xfffful in
+  let sum11 = UInt32.add_mod (sum1 &^ 0xfffful) (sum1 >>^ 16ul) in
+  let sum21 = UInt32.add_mod (sum2 &^ 0xfffful) (sum2 >>^ 16ul) in
+  (sum21 <<^ 16ul) |^ sum11
